Restructuring of Interfaces; more show cases.

thys/Isabelle_C/C11-FrontEnd/src/C_Command.thy
@@ -145,7 +145,108 @@ end
 \<close>
 
 ML \<comment> \<open>\<^theory>\<open>Isabelle_C.C_Eval\<close>\<close> \<open>
-structure C_Module =
+
+signature C_MODULE =
+ sig
+    structure Data_Accept    : GENERIC_DATA
+    structure Data_In_Env    : GENERIC_DATA
+    structure Data_In_Source : GENERIC_DATA
+    structure Data_Term      : GENERIC_DATA
+
+    structure C_Term:
+      sig
+        val key0_default: string
+        val key0_expression: string
+        val key0_external_declaration: string
+        val key0_statement: string
+        val key0_translation_unit: string
+        val key_default: Input.source
+        val key_expression: Input.source
+        val key_external_declaration: Input.source
+        val key_statement: Input.source
+        val key_translation_unit: Input.source
+        val map_default: (C_Grammar_Rule.start_happy -> C_Env.env_lang -> local_theory -> term) -> theory -> theory
+        val map_expression: (C_Grammar_Rule_Lib.CExpr -> C_Env.env_lang -> local_theory -> term) -> theory -> theory
+        val map_external_declaration:
+           (C_Grammar_Rule_Lib.CExtDecl -> C_Env.env_lang -> local_theory -> term) -> theory -> theory
+        val map_statement: (C_Grammar_Rule_Lib.CStat -> C_Env.env_lang -> local_theory -> term) -> theory -> theory
+        val map_translation_unit:
+           (C_Grammar_Rule_Lib.CTranslUnit -> C_Env.env_lang -> local_theory -> term) -> theory -> theory
+        val tok0_expression: string * ('a * 'a -> (C_Grammar.Tokens.svalue, 'a) LALR_Parser_Eval.Token.token)
+        val tok0_external_declaration: string * ('a * 'a -> (C_Grammar.Tokens.svalue, 'a) LALR_Parser_Eval.Token.token)
+        val tok0_statement: string * ('a * 'a -> (C_Grammar.Tokens.svalue, 'a) LALR_Parser_Eval.Token.token)
+        val tok0_translation_unit: string * ('a * 'a -> (C_Grammar.Tokens.svalue, 'a) LALR_Parser_Eval.Token.token)
+        val tok_expression: Input.source * ('a * 'a -> (C_Grammar.Tokens.svalue, 'a) LALR_Parser_Eval.Token.token)
+        val tok_external_declaration: Input.source * ('a * 'a -> (C_Grammar.Tokens.svalue, 'a) LALR_Parser_Eval.Token.token)
+        val tok_statement: Input.source * ('a * 'a -> (C_Grammar.Tokens.svalue, 'a) LALR_Parser_Eval.Token.token)
+        val tok_translation_unit: Input.source * ('a * 'a -> (C_Grammar.Tokens.svalue, 'a) LALR_Parser_Eval.Token.token)
+        val tokens: (string * ('a * 'a -> (C_Grammar.Tokens.svalue, 'a) LALR_Parser_Eval.Token.token)) list
+      end
+    structure C_Term':
+      sig
+        val accept:
+           local_theory ->
+             (Input.source * (Position.range -> (C_Grammar.Tokens.svalue, Position.T) LALR_Parser_Eval.Token.token)) option ->
+               (Input.source -> Context.generic -> (C_Grammar.Tokens.svalue, Position.T) LALR_Parser_Eval.Token.token) *
+               (Data_In_Env.T ->
+                  'a * (C_Grammar_Rule.start_happy * 'b * 'c) ->
+                    {context: Context.generic, error_lines: 'd, reports_text: 'e} ->
+                      term * {context: Context.generic, error_lines: 'd, reports_text: 'e})
+        val err:
+           C_Env.env_lang ->
+             (LALR_Table.state * (C_Grammar_Parser.svalue0 * Position.T * Position.T)) list ->
+               Position.T ->
+                 {context: Context.generic, error_lines: string list, reports_text: Position.report_text list} ->
+                   term * {context: Context.generic, error_lines: string list, reports_text: Position.report_text list}
+        val eval_in:
+           Input.source ->
+             Context.generic ->
+               (Context.generic ->
+                  C_Env.env_lang) ->
+                 (Input.source * (Position.range -> (C_Grammar.Tokens.svalue, Position.T) LALR_Parser_Eval.Token.token)) option
+                   -> C_Lex.token list * (C_Env.error_lines -> string list) -> term
+        val parse_translation:
+           ('a * (Input.source * (Position.range -> (C_Grammar.Tokens.svalue, Position.T) LALR_Parser_Eval.Token.token)) option)
+           list
+             -> ('a * (Proof.context -> term list -> term)) list
+      end
+
+    val C: Input.source -> Context.generic -> generic_theory
+    val C': C_Env.env_lang -> Input.source -> Context.generic -> Context.generic
+
+    val C_export_boot: Input.source -> Context.generic -> generic_theory
+    val C_export_file: Position.T * 'a -> Proof.context -> Proof.context
+    val C_prf: Input.source -> Proof.state -> Proof.state
+    val accept:
+       Data_In_Env.T ->
+         'a * (C_Grammar_Rule.start_happy * 'b * 'c) ->
+           {context: Context.generic, error_lines: 'd, reports_text: 'e} ->
+             unit * {context: Context.generic, error_lines: 'd, reports_text: 'e}
+    val accept0:
+       (Context.generic -> C_Grammar_Rule.start_happy -> Data_In_Env.T -> Context.generic -> 'a) ->
+         Data_In_Env.T -> C_Grammar_Rule.start_happy -> Context.generic -> 'a
+    val c_enclose: string -> string -> Input.source -> C_Lex.token list * (string list -> string list)
+    val env: Context.generic -> Data_In_Env.T
+    val env0: Proof.context -> Data_In_Env.T
+    val err:
+       C_Env.env_lang ->
+         (LALR_Table.state * (C_Grammar_Parser.svalue0 * Position.T * Position.T)) list ->
+           Position.T ->
+             {context: Context.generic, error_lines: string list, reports_text: Position.report_text list} ->
+               unit * {context: Context.generic, error_lines: string list, reports_text: Position.report_text list}
+    val err0:
+       'a ->
+         'b ->
+           Position.T ->
+             {context: 'c, error_lines: string list, reports_text: 'd} ->
+               {context: 'c, error_lines: string list, reports_text: 'd}
+    val eval_in: Input.source -> Context.generic option -> C_Lex.token list * (C_Env.error_lines -> string list) -> unit
+    val eval_source: Input.source -> unit
+    val exec_eval: Input.source -> Context.generic -> Context.generic
+    val start: Input.source -> Context.generic -> (C_Grammar.Tokens.svalue, Position.T) LALR_Parser_Eval.Token.token
+  end
+
+structure C_Module : C_MODULE =
 struct
 
 structure Data_In_Source = Generic_Data
@@ -172,35 +273,36 @@ structure Data_Term = Generic_Data
    val extend = I
    val merge = #2)
 
+
 structure C_Term =
 struct
-val key_translation_unit = \<open>translation_unit\<close>
-val key_external_declaration = \<open>external_declaration\<close>
-val key_statement = \<open>statement\<close>
-val key_expression = \<open>expression\<close>
-val key_default = \<open>default\<close>
+   val key_translation_unit     = \<open>translation_unit\<close>
+   val key_external_declaration = \<open>external_declaration\<close>
+   val key_statement            = \<open>statement\<close>
+   val key_expression           = \<open>expression\<close>
+   val key_default              = \<open>default\<close>
 
 local
-val source_content = Input.source_content #> #1
+   val source_content = Input.source_content #> #1
 in
-val key0_translation_unit = source_content key_translation_unit
-val key0_external_declaration = source_content key_external_declaration
-val key0_statement = source_content key_statement
-val key0_expression = source_content key_expression
-val key0_default = source_content key_default
+   val key0_translation_unit = source_content key_translation_unit
+   val key0_external_declaration = source_content key_external_declaration
+   val key0_statement = source_content key_statement
+   val key0_expression = source_content key_expression
+   val key0_default = source_content key_default
 end
 
-val tok0_translation_unit = (key0_translation_unit, C_Grammar.Tokens.start_translation_unit)
+val tok0_translation_unit     = (key0_translation_unit, C_Grammar.Tokens.start_translation_unit)
 val tok0_external_declaration = ( key0_external_declaration
                                 , C_Grammar.Tokens.start_external_declaration)
-val tok0_statement = (key0_statement, C_Grammar.Tokens.start_statement)
-val tok0_expression = (key0_expression, C_Grammar.Tokens.start_expression)
+val tok0_statement            = (key0_statement, C_Grammar.Tokens.start_statement)
+val tok0_expression           = (key0_expression, C_Grammar.Tokens.start_expression)
 
-val tok_translation_unit = (key_translation_unit, C_Grammar.Tokens.start_translation_unit)
-val tok_external_declaration = ( key_external_declaration
-                               , C_Grammar.Tokens.start_external_declaration)
-val tok_statement = (key_statement, C_Grammar.Tokens.start_statement)
-val tok_expression = (key_expression, C_Grammar.Tokens.start_expression)
+val tok_translation_unit      = (key_translation_unit, C_Grammar.Tokens.start_translation_unit)
+val tok_external_declaration  = ( key_external_declaration
+                                , C_Grammar.Tokens.start_external_declaration)
+val tok_statement             = (key_statement, C_Grammar.Tokens.start_statement)
+val tok_expression            = (key_expression, C_Grammar.Tokens.start_expression)
 
 val tokens = [ tok0_translation_unit
              , tok0_external_declaration
@@ -243,11 +345,11 @@ fun err0 _ _ pos =
 
 val err = pair () oooo err0
 
-fun accept0 f env_lang ast =
+fun accept0 f (env_lang:C_Env.env_lang) ast =
   Data_In_Env.put env_lang
   #> (fn context => f context ast env_lang (Data_Accept.get context ast env_lang context))
 
-fun accept env_lang (_, (ast, _, _)) =
+fun accept (env_lang:C_Env.env_lang) (_, (ast, _, _)) =
   pair () o C_Env.map_context (accept0 (K (K (K I))) env_lang ast)
 
 val eval_source = C_Context.eval_source env start err accept
@@ -350,11 +452,13 @@ fun C_export_boot source context =
   |> Config.restore_generic ML_Env.ML_environment context
   |> Local_Theory.propagate_ml_env
 
-fun C source =
-  exec_eval source
-  #> Local_Theory.propagate_ml_env
+val C: Input.source -> Context.generic -> Context.generic  = 
+       fn source => 
+                    exec_eval source
+                    #> Local_Theory.propagate_ml_env
 
-fun C' env_lang src context =
+val C': C_Env.env_lang -> Input.source -> Context.generic -> Context.generic  =
+    fn env_lang:C_Env.env_lang => fn src:Input.source => fn context:Context.generic =>
   context
   |> C_Env.empty_env_tree
   |> C_Context.eval_source'
@@ -366,7 +470,7 @@ fun C' env_lang src context =
   |> (fn (_, {context, reports_text, error_lines}) => 
      tap (fn _ => case error_lines of [] => () | l => warning (cat_lines (rev l)))
          (C_Stack.Data_Tree.map (curry C_Stack.Data_Tree_Args.merge (reports_text, []))
-                                context))
+                                 context))
 
 fun C_export_file (pos, _) lthy =
   let
@@ -397,7 +501,14 @@ subsection \<open>Definitions of Inner Directive Commands\<close>
 subsubsection \<open>Initialization\<close>
 
 ML \<comment> \<open>\<^theory>\<open>Pure\<close>\<close> \<open>
-structure C_Directive =
+structure C_Directive :
+ sig
+    val setup_define:
+       Position.T ->
+         (C_Lex.token list -> string * Position.range -> Context.generic 
+          -> C_Lex.token list * Context.generic) ->
+           (string * Position.range -> Context.generic -> Context.generic) -> theory -> theory
+  end =
 struct
 local
 fun directive_update keyword data = C_Context.directive_update keyword (data, K (K (K I)))
@@ -959,5 +1070,32 @@ C_Module.C_Term'.parse_translation
   , (\<^syntax_const>\<open>_C_statement\<close>, SOME C_Module.C_Term.tok_statement)
   , (\<^syntax_const>\<open>_C\<close>, NONE) ]
 \<close>
+ML\<open> Context.the_generic_context()\<close>
+ML\<open>@{context}\<close>
+ML\<open>C_Module.env (Context.the_generic_context())\<close>
+ML\<open>
+ML_Antiquotation.value_embedded;
+Theory.check;
+\<close>
+
+subsection\<open>ML-Antiquotations as Programming Support\<close>
+
+ML\<open>
+val _ = Theory.setup(
+  ML_Antiquotation.value_embedded \<^binding>\<open>C\<^sub>e\<^sub>n\<^sub>v\<close>
+    (Args.context -- Scan.lift Args.embedded_position >> (fn (ctxt, (name, pos)) =>
+      (warning"arg variant not implemented";"C_Module.env (Context.the_generic_context())"))
+    || Scan.succeed "C_Module.env (Context.the_generic_context())"))
+
+\<close>
+
+text\<open>Note that this anti-quotation is controlled by the \<^verbatim>\<open>C_starting_env\<close> - flag.  \<close>    
+
+declare[[C\<^sub>e\<^sub>n\<^sub>v\<^sub>0 = last]]
+ML\<open>@{C\<^sub>e\<^sub>n\<^sub>v}\<close>
+
+declare[[C\<^sub>e\<^sub>n\<^sub>v\<^sub>0 = empty]]
+ML\<open>@{C\<^sub>e\<^sub>n\<^sub>v}\<close>
+
 
 end
